[jvm] Strengthen invariants over the JVM state.
The call-stack contains only well-formed frames.
Frames cannot represent native or abstract methods.
The PC in the frame must be valid wrt the program (must be the location of the start of an instruction).

Also adapt Axe as needed.

books/kestrel/jvm/frames.lisp
@@ -1,7 +1,7 @@
 ; Call stack frames
 ;
 ; Copyright (C) 2008-2011 Eric Smith and Stanford University
-; Copyright (C) 2013-2021 Kestrel Institute
+; Copyright (C) 2013-2026 Kestrel Institute
 ;
 ; License: A 3-clause BSD license. See the file books/3BSD-mod.txt.
 ;
@@ -23,6 +23,8 @@
 (local (include-book "kestrel/lists-light/cdr" :dir :system))
 (local (include-book "kestrel/lists-light/cons" :dir :system))
 
+(local (in-theory (disable method-program)))
+
 (defund maybe-addressp (item)
   (declare (xargs :guard t))
   (or (acl2::addressp item)
@@ -36,17 +38,22 @@
 ;; same as the method-info stored in the class table, but I suppose we don't
 ;; know that a priori.
 
+;; Recognizes a well-formed frame on the call-stack.
 ;fixme uncomment things below and flesh out
 (defund framep (frame)
   (declare (xargs :guard t))
   (and (true-listp frame)
        (equal (len frame) 6)
-       (pcp (nth 0 frame)) ;the pc (fixme also must point to an instruction within the program)
+       (pcp (nth 0 frame))        ;the pc
        (true-listp (nth 1 frame)) ; todo: what else to say about the locals?
        (operand-stackp (nth 2 frame)) ; todo: what else to say about the operand stack?
        (maybe-addressp (nth 3 frame)) ;the locked-object
        (method-infop (nth 4 frame))
-       (method-designatorp (nth 5 frame))))
+       (method-designatorp (nth 5 frame))
+       (not (method-abstractp (nth 4 frame))) ; if the method was native or abstract we wouldn't even have a frame with a PC, etc.
+       (not (method-nativep (nth 4 frame)))
+       ;; the PC points to an instruction within the program:
+       (if (member-equal (nth 0 frame) (strip-cars (method-program (nth 4 frame)))) t nil)))
 
 ;Now includes the class name and method name (and descriptor) of the method being invoked (nice to have this info in the trace and for debugging):
 (defund make-frame (pc     ;; program counter
@@ -57,7 +64,7 @@
                     method-info ;;a method-infop (includes static flag, syn flag, program, exception table, etc.)
                     method-designator ; this info isn't used for much (fixme think through the calls of (cur-xxx... ) below. update: now is used by invokespecial!
                     )
-  (declare (type t pc locals stack locked-object method-info method-designator))
+  (declare (type t pc locals stack locked-object method-info method-designator)) ; todo: strengthen
   (list pc locals stack locked-object method-info method-designator))
 
 (defthm framep-of-make-frame
@@ -67,7 +74,10 @@
               (operand-stackp stack)
               (maybe-addressp locked-object)
               (method-infop method-info)
-              (method-designatorp method-designator)))
+              (method-designatorp method-designator)
+              (not (method-abstractp method-info))
+              (not (method-nativep method-info))
+              (if (member-equal pc (strip-cars (method-program method-info))) t nil)))
   :hints (("Goal" :in-theory (enable framep make-frame))))
 
 (defthm equal-of-make-frame-and-make-frame
@@ -207,3 +217,18 @@
   (implies (framep frame)
            (method-descriptorp (cur-method-descriptor frame)))
   :hints (("Goal" :in-theory (enable framep cur-method-descriptor method-designatorp method-descriptorp method-designator))))
+
+(defthm not-method-nativep-of-method-info-when-framep
+  (implies (framep frame)
+           (not (method-nativep (method-info frame))))
+  :hints (("Goal" :in-theory (enable framep method-info))))
+
+(defthm not-method-abstractp-of-method-info-when-framep
+  (implies (framep frame)
+           (not (method-abstractp (method-info frame))))
+  :hints (("Goal" :in-theory (enable framep method-info))))
+
+(defthm instructionp-of-lookup-equal-of-pc-and-method-program-of-method-info
+  (implies (framep frame)
+           (instructionp (lookup-equal (pc frame) (method-program (method-info frame)))))
+  :hints (("Goal" :in-theory (enable framep method-infop method-info method-access-flags pc pcp))))
